checker/theories/Closed.v
@@ -428,7 +428,7 @@ Lemma declared_decl_closed `{checker_flags} (Σ : global_env) cst decl :
   wf Σ ->
   lookup_env Σ cst = Some decl ->
   on_global_decl (fun Σ Γ b t => closedn #|Γ| b && option_default (closedn #|Γ|) t true)
-                 (Σ, universes_decl_of_decl decl) decl.
+                 (Σ, universes_decl_of_decl decl) cst decl.
 Proof.
   intros.
   eapply weaken_lookup_on_global_env; try red; eauto.
