pcuic/theories/PCUICNormal.v
@@ -50,7 +50,7 @@ Section Normal.
   | ne_var v : neutral Γ (tVar v)
   | ne_evar n l : neutral Γ (tEvar n l)
   | ne_const c u decl :
-      lookup_env Σ c = Some (ConstantDecl c decl) -> decl.(cst_body) = None ->
+      lookup_env Σ c = Some (ConstantDecl decl) -> decl.(cst_body) = None ->
       neutral Γ (tConst c u)
   | ne_app f v : neutral Γ f -> normal Γ v -> neutral Γ (tApp f v)
   | ne_case i p c brs : neutral Γ c -> Forall (compose (normal Γ) snd) brs ->
@@ -88,7 +88,7 @@ Section Normal.
       whne Γ (tLetIn na B b t)
 
   | whne_const c u decl :
-      lookup_env Σ c = Some (ConstantDecl c decl) ->
+      lookup_env Σ c = Some (ConstantDecl decl) ->
       decl.(cst_body) = None ->
       whne Γ (tConst c u)
 
